coq/src/Sets.v
@@ -3,98 +3,48 @@ Set Asymmetric Patterns.
 
 Require Export Ensembles Finite_sets Finite_sets_facts.
 
-Ltac sig_auto :=
-  repeat match goal with
-  | [ H: { _ : _ | _ } |- _ ] => destruct H
-  end; auto.
+Require Import Tapl.Tactics.
+From Ltac2 Require Import Ltac2 Notations.
+From Ltac2 Require Control.
 
-Ltac conj_disj_elim tac :=
-  repeat match goal with
-    | [ H: _ \/ _ |- _ ] => destruct H
-    | [ H: _ /\ _ |- _ ] => destruct H
-    | [ |- _ /\ _ ] => split
-    | [ |- _ \/ _ ] => (left; progress tac) || (right; progress tac) || idtac
-    end.
+Ltac2 rec union_search (tac: unit -> unit) :=
+    let app t := apply (ltac2:(t)); orelse (fun _ => progress (tac ())) (fun _ => union_search tac) in
+    app (constr:(Union_introl)) || app (constr:(Union_intror)).
 
-Ltac sets_basic :=
-  intros;
-  match goal with
-  | [ |- _ = _ ] => apply Extensionality_Ensembles
-  | [ |- ~ _ ] => intro
-  | [ |- context[In _ (Singleton _ _) _] ] => apply In_singleton
-  | [ |- context[Couple _ _ _] ] => rewrite <- Couple_as_union
-  | [ |- context[Triple _ _ _ _] ] => rewrite <- Triple_as_union
-  | [ H: In _ (Singleton _ _) _ |- _ ] => inversion H
-  | [ H: In _ (Couple _ _ _) _ |- _ ] => inversion H
-  | [ H: In _ (Triple _ _ _ _) _ |- _ ] => inversion H
-  | [ H: In _ (Union _ _ _) _ |- _ ] => inversion H
-  end;
-  repeat (unfold Same_set in * || unfold Included in * );
-  eauto with sets;
-  firstorder.
-
-Ltac search_union tac :=
-  let rec search := tac ||
-    match goal with
-    | [ |- In _ (Union _ _ _) _ ] =>
-        progress tac
-        || (apply Union_introl; search)
-        || (apply Union_intror; search)
-    end in
-  repeat search.
-
-Ltac search_couple tac :=
-  let rec search := tac ||
-    match goal with
-    | [ |- In _ (Couple _ _ _) _ ] =>
-        progress tac
-        || (apply Couple_l; search)
-        || (apply Couple_r; search)
-    end in
-  repeat search.
-
-Ltac search_triple tac :=
-  let rec search := tac ||
-    match goal with
-    | [ |- In (Triple _ _ _ _) _ ] =>
-        progress tac
-        || (apply Triple_l; search)
-        || (apply Triple_m; search)
-        || (apply Triple_r; search)
-    end in
-  repeat search.
+Ltac2 rec sets_basic0 () :=
+    Control.enter (fun _ => intros; repeat (match! goal with
+    | [ |- _ = _ ] =>
+        apply Extensionality_Ensembles;
+        unfold Same_set; unfold Included;
+        split; intros
+    | [ |- ~ _ ] => unfold not; intro
+    | [ |- In _ (Singleton _ _) _ ] => apply In_singleton
+    | [ |- context[Couple _ _ _] ] => rewrite <- Couple_as_union
+    | [ |- context[Triple _ _ _ _] ] => rewrite <- Triple_as_union
+    | [ h: In _ (Singleton _ _) _ |- _ ] => rawinversion_clear h
+    | [ h: In _ (Couple _ _ _) _ |- _ ] => rawinversion_clear h
+    | [ h: In _ (Triple _ _ _ _) _ |- _ ] => rawinversion_clear h
+    | [ |- context[Add _ (Empty_set _) _] ] => rewrite Empty_set_zero'
+    | [ h: context[Add _ (Empty_set _) _] |- _] => rewrite Empty_set_zero' in *
+    end);
+    auto with sets).
+Ltac2 Notation sets_basic := sets_basic0 ().
 
 Section sets.
   Variable U: Type.
   Variable x y z: U.
 
-  Ltac solve :=
-    sets_basic;
-    rewrite Empty_set_zero' in *;
-    unfold Add in *;
-    repeat match goal with
-    | [ H: In _ (Singleton _ _) _ |- _ ] => inversion H; clear H
-    | [ H: In _ (Couple _ _ _) _ |- _ ] => inversion H; clear H
-    | [ H: In _ (Triple _ _ _ _) _ |- _ ] => inversion H; clear H
-    | [ H: In _ (Union _ _ _) _ |- _ ] => inversion H; clear H
-    end;
-    match goal with
-    | [ |- context[Singleton] ] => apply In_singleton
-    | [ |- context[Couple] ] => search_couple ltac:(solve)
-    | [ |- context[Triple] ] => search_triple ltac:(solve)
-    | [ |- context[Union] ] => search_union ltac:(solve)
-    end.
-
   Lemma Singleton_Add: Singleton _ x = Add _ (Empty_set _) x.
-  Proof. solve. Qed.
+  Proof. sets_basic. Qed.
 
   Lemma Couple_Add: Couple _ x y = Add _ (Add _ (Empty_set _) x) y.
-  Proof. solve. Qed.
+  Proof. sets_basic. Qed.
 
   Lemma Triple_Add: Triple _ x y z = Add _ (Add _ (Add _ (Empty_set _) x) y) z.
-  Proof. solve. Qed.
+  Proof. sets_basic. Qed.
 End sets.
 
+(*
 Ltac sets_rewrite tac :=
   match goal with
   | [ |- context[Union _ (Union _ _ _) _] ] => rewrite Union_associative; progress tac
@@ -116,6 +66,7 @@ Ltac sets_auto :=
     eauto with sets);
   try sets_rewrite sets_basic;
   eauto with sets.
+*)
 
 Notation "'Yes'" := (left _).
 Notation "'No'" := (right _).
