coq/src/Tactics.v
@@ -1,0 +1,80 @@
+From Ltac2 Require Import Ltac2 Notations.
+From Ltac2 Require Message String Char List Std Control.
+
+Ltac2 msg_string s := Message.of_string s.
+Ltac2 msg_int n := Message.of_int n.
+Ltac2 msg_ident id := Message.of_ident id.
+Ltac2 msg_constr c := Message.of_constr c.
+Ltac2 msg_exn e := Message.of_exn e.
+
+Ltac2 Notation a(self) ":+:" b(self) := Message.concat a b.
+
+Ltac2 msg_char c := msg_string (String.make 1 c).
+Ltac2 newline0 () := msg_char (Char.of_int 10).
+Ltac2 Notation newline := newline0 ().
+
+Ltac2 print := Message.print.
+Ltac2 println m := Message.print (m :+: newline).
+
+Ltac2 print_string s := print (msg_string s).
+Ltac2 println_string s := println (msg_string s).
+Ltac2 print_int n := print (msg_int n).
+Ltac2 println_int n := println (msg_int n).
+Ltac2 print_ident id := print (msg_ident id).
+Ltac2 println_ident id := println (msg_ident id).
+Ltac2 print_constr c := print (msg_constr c).
+Ltac2 println_constr c := println (msg_constr c).
+Ltac2 print_exn e := print (msg_exn e).
+Ltac2 println_exn e := println (msg_exn e).
+
+Ltac2 msg_fold ms := List.fold_left (Message.concat) ms (msg_string "").
+
+Ltac2 msg_join (m: message) (ms: message list) :=
+    let rec msg_join' ms := match ms with
+    | [] => []
+    | h :: t => match t with
+        | [] => h :: []
+        | _ :: _ => h :: m :: msg_join' t
+        end
+    end in
+    let ms' := msg_join' ms
+    in msg_fold ms'.
+
+Ltac2 msg_lines ms := msg_join newline ms.
+
+Ltac2 Notation "simple" "rawinversion"
+    arg(self)
+    pat(opt(seq("as", intropattern)))
+    ids(opt(seq("in", list1(ident)))) :=
+    Std.inversion Std.SimpleInversion (Std.ElimOnIdent arg) pat ids.
+
+Ltac2 Notation "rawinversion"
+    arg(self)
+    pat(opt(seq("as", intropattern)))
+    ids(opt(seq("in", list1(ident)))) :=
+    Std.inversion Std.FullInversion (Std.ElimOnIdent arg) pat ids.
+
+Ltac2 Notation "rawinversion_clear"
+    arg(self)
+    pat(opt(seq("as", intropattern)))
+    ids(opt(seq("in", list1(ident)))) :=
+    Std.inversion Std.FullInversionClear (Std.ElimOnIdent arg) pat ids.
+
+Ltac2 alternation (a: unit -> unit) (b: unit -> unit) :=
+    Control.plus a (fun _ => b ()).
+
+Ltac2 Notation a(self) "||" b(self) := alternation (fun _ => a) (fun _ => b).
+
+Ltac2 sig_auto0 () :=
+    repeat (match! goal with
+        | [ h: { _ : _ | _ } |- _ ] => destruct h
+        end); auto.
+Ltac2 Notation sig_auto := sig_auto0 ().
+
+Ltac2 conj_disj_elim tac :=
+    repeat (match! goal with
+        | [ h: _ /\ _ |- _ ] => destruct h
+        | [ h: _ \/ _ |- _ ] => destruct h
+        | [ |- _ /\ _ ] => split
+        | [ |- _ \/ _ ] => (left; progress tac) || (right; progress tac) || ()
+        end); auto.
